WIP adapting step_async

Wavelet/Compile/AffineChan.lean
@@ -7,7 +7,6 @@ open Semantics
 def AtomicProc.inputs [Arity Op] : AtomicProc Op χ V → List χ
   | .op _ inputs _ => inputs.toList
   | .async _ inputs _ => inputs.toList
-  | .switch _ inputs _ _ => inputs.toList
   | .steer _ _ inputs _ => inputs.toList
   | .carry _ _ inputs₁ inputs₂ _ => (inputs₁ ++ inputs₂).toList
   | .merge _ inputs₁ inputs₂ _ => (inputs₁ ++ inputs₂).toList
@@ -20,7 +19,6 @@ def AtomicProc.inputs [Arity Op] : AtomicProc Op χ V → List χ
 def AtomicProc.outputs [Arity Op] : AtomicProc Op χ V → List χ
   | .op _ _ outputs => outputs.toList
   | .async _ _ outputs => outputs.toList
-  | .switch _ _ outputs₁ outputs₂ => (outputs₁ ++ outputs₂).toList
   | .steer _ _ _ outputs => outputs.toList
   | .carry _ _ _ _ outputs => outputs.toList
   | .merge _ _ _ outputs => outputs.toList
